strong pullback preservation not needed when no live left

operations/Linearize.thy
@@ -12,6 +12,27 @@ to be pullback-preserving), we transform it into an MRBNF F' that has the same c
 as F except that the 3rd position becomes map-constrained to small-support endobijections.  
 *)
 
+text \<open>
+
+rail\<open>
+  @@{command linearize_mrbnf} @{syntax spec} name '=' term @{syntax wits}? @'on' @{syntax on_vars} @{syntax bindings}? @{syntax morphisms}?
+  ;
+  @{syntax_def spec}: @{syntax tfree} | '(' (((name ':')? @{syntax tfree}) + ',') ')'
+  ;
+  @{syntax_def tfree}: typefree ('::' sort)
+  ;
+  @{syntax_def wits}: '[' 'wits' ':' (term + ',') ']'
+  ;
+  @{syntax_def on_vars}: (typefree + @'and')
+  ;
+  @{syntax_def bindings}: @'for' ((('map' | 'rel' | 'pred' | 'nonrep' | 'sameShape') ':' name) +)
+  ;
+  @{syntax_def morphisms}: @'morphisms' name name
+\<close>
+
+\<close>
+
+
 definition asSS :: "('a \<Rightarrow> 'a) \<Rightarrow> 'a \<Rightarrow> 'a" where
   "asSS f \<equiv> if |supp f| <o |UNIV :: 'a set| then f else id"
 
@@ -39,13 +60,28 @@ ML \<open>val lin_pos = 3\<close>
 
 print_mrbnfs
 declare [[ML_print_depth=10000]]
-ML \<open>MRBNF_Def.mrbnf_of @{context} @{type_name F} |> the \<close>
+
+thm F.in_rel[OF supp_id_bound bij_id supp_id_bound, unfolded F.map_id]
+
+lemma "rrel_F R S x y =
+      (\<exists>!z. set3_F z \<subseteq> {(x, y). R x y} \<and>
+            set4_F z \<subseteq> {(x, y). S x y} \<and> map_F id id fst fst z = x \<and> map_F id id snd snd z = y)"
+  apply (rule iffI)
+   prefer 2
+   apply (drule ex1_implies_ex)
+  apply (erule F.in_rel[OF supp_id_bound bij_id supp_id_bound, unfolded F.map_id, THEN iffD2, unfolded mem_Collect_eq conj_assoc])
+  apply (rule ex_ex1I)
+   apply (erule F.in_rel[OF supp_id_bound bij_id supp_id_bound, unfolded F.map_id, THEN iffD1, unfolded mem_Collect_eq conj_assoc])
+  apply (elim conjE)
+  subgoal for z z'
+    apply (hypsubst_thin)
+    oops
 
 axiomatization where
   (* The next property assumes preservation of pullbacks on the third position. 
    NB: All MRBNFs already preserve _weak_ pullbacks, i.e., they satisfy the following property 
    without uniqueness.  *)
-  F_rel_map_set2_strong: 
+  F_rel_map_set_live_strong: 
   "\<And> R S (x :: ('a :: var,'b :: var,'c,'d) F) y.
     rrel_F R S x y =
       (\<exists>!z. set3_F z \<subseteq> {(x, y). R x y} \<and>
@@ -58,138 +94,128 @@ abbreviation "rel_F \<equiv> mr_rel_F"
 
 (* Important consequence of preservation of pullbacks (which is actually equivalent to it): 
 The relator is closed under intersections. *)
-
-ML \<open>
-open BNF_Util BNF_Tactics MRBNF_Def
-
-fun mk_F_strong_tac mrbnf F_map_id mr_rel_F_def F_mr_rel_mono_strong0 F_rel_map_set2_strong F_in_rel ctxt =
-  let
-    val id_prems = MRBNF_Comp_Tactics.mk_id_prems mrbnf;
-    val var_types = var_types_of_mrbnf mrbnf;
-    val nr_lives = length (filter (fn v => v = MRBNF_Def.Live_Var) var_types);
-  in
-    HEADGOAL (
-      forward_tac ctxt [F_mr_rel_mono_strong0 OF flat (replicate 2 id_prems)] THEN_ALL_NEW (
-        TRY o (rtac ctxt ballI THEN_ALL_NEW 
-          resolve_tac ctxt [ballI, refl]) THEN_ALL_NEW
-        TRY o (rtac ctxt impI THEN_ALL_NEW
-          rtac ctxt (trans OF [@{thm top_apply} RS fun_cong, trans OF @{thms top_apply top_bool_def}])))) THEN
-    unfold_thms_tac ctxt [F_map_id, mr_rel_F_def, @{thm eq_True}] THEN
-    HEADGOAL (rotate_tac 2) THEN
-    HEADGOAL (dtac ctxt (iffD1 OF [F_rel_map_set2_strong])) THEN
-    unfold_thms_tac ctxt ([eqTrueI OF [subset_UNIV]] @ @{thms top_apply top_bool_def 
-      Collect_const_case_prod if_True simp_thms(22)}) THEN
-    unfold_thms_tac ctxt ([unfold_thms ctxt [id_apply, F_map_id, @{thm OO_Grp_alt}] (F_in_rel OF 
-      id_prems), sym OF @{thms id_def}, mem_Collect_eq]) THEN
-    HEADGOAL (etac ctxt exE) THEN
-    HEADGOAL (etac ctxt exE) THEN
-    HEADGOAL (etac ctxt @{thm alt_ex1E}) THEN
-    REPEAT_DETERM_N (3+2*nr_lives) (HEADGOAL (etac ctxt conjE)) THEN
-    HEADGOAL (Subgoal.FOCUS
-      (fn {prems, context = ctxt, params, ...} => 
-        HEADGOAL (Method.insert_tac ctxt [
-          infer_instantiate' ctxt [SOME (snd (nth params 1)), SOME (snd (nth params 0))] (@{thm spec2} OF [nth prems 0]),
-          infer_instantiate' ctxt [SOME (snd (nth params 2)), SOME (snd (nth params 0))] (@{thm spec2} OF [nth prems 0])] THEN_ALL_NEW
-          etac ctxt impE THEN_ALL_NEW
-          etac ctxt impE) THEN
-        REPEAT_DETERM_N 3 (HEADGOAL (
-          rtac ctxt conjI THEN_ALL_NEW
-          rtac ctxt conjI THEN_ALL_NEW
-          resolve_tac ctxt prems)) THEN
-        HEADGOAL (rtac ctxt exI) THEN
-        unfold_thms_tac ctxt @{thms inf_fun_def inf_bool_def} THEN
-        HEADGOAL (rtac ctxt conjI) THEN
-        HEADGOAL (Method.insert_tac ctxt prems) THEN
-        HEADGOAL (hyp_subst_tac_thin true ctxt) THEN
-        REPEAT_DETERM_N nr_lives (HEADGOAL (EVERY' [
-          TRY o rtac ctxt conjI,
-          rtac ctxt @{thm subrelI},
-          rtac ctxt CollectI,
-          rtac ctxt @{thm case_prodI},
-          rtac ctxt conjI THEN_ALL_NEW 
-            etac ctxt (@{thm rev_subsetD} RS (iffD1 OF @{thms prod_in_Collect_iff})),
-        assume_tac ctxt,
-        assume_tac ctxt])) THEN
-        HEADGOAL (rtac ctxt conjI THEN_ALL_NEW resolve_tac ctxt prems)
-      ) ctxt)
-  end
-\<close>
-
-(* lin_pos independent *)
 lemma F_strong:
   "rel_F id id R3 R4 x y \<Longrightarrow> rel_F id id Q3 Q4 x y \<Longrightarrow> rel_F id id (inf R3 Q3) (inf R4 Q4) x y"
-  apply (tactic \<open>mk_F_strong_tac (MRBNF_Def.mrbnf_of @{context} @{type_name F} |> the) @{thm F.map_id} 
-    @{thm mr_rel_F_def} @{thm F.mr_rel_mono_strong0} @{thm F_rel_map_set2_strong} @{thm F.in_rel} @{context} 
-    THEN print_tac @{context} "done" THEN no_tac\<close>)
-
   apply (frule F.mr_rel_mono_strong0[OF supp_id_bound bij_id supp_id_bound supp_id_bound bij_id supp_id_bound];
       ((rule ballI, rule ballI refl)?, 
         (rule impI, rule trans[OF top_apply[THEN fun_cong] trans[OF top_apply top_bool_def]])?)) 
-  thm trans[OF top_apply[THEN fun_cong] trans[OF top_apply top_bool_def]]
-  apply(rotate_tac 2)
   apply (unfold F.map_id mr_rel_F_def eq_True)
-  thm F_rel_map_set2_strong
-  apply (drule F_rel_map_set2_strong[THEN iffD1])
+  apply (rotate_tac 2)
+  apply (drule F_rel_map_set_live_strong[THEN iffD1])
   apply (unfold top_apply top_bool_def Collect_const_case_prod if_True eqTrueI[OF subset_UNIV] simp_thms(22))
   apply (unfold F.in_rel[OF supp_id_bound bij_id supp_id_bound, unfolded id_apply F.map_id OO_Grp_alt]
       id_def[symmetric] mem_Collect_eq)
-  apply (elim exE alt_ex1E)
-  apply (erule conjE)
-  apply (erule conjE)
-  apply (erule conjE)
-  apply (erule conjE)
-  apply (erule conjE)
-  apply (erule conjE)
-  apply (erule conjE)
-  subgoal premises subprems for z l r
-    thm subprems
-    apply (insert spec2[OF subprems(1), of r z]
-        spec2[OF subprems(1), of l z]; (erule impE); (erule impE))
-       apply (rule conjI; rule conjI; rule subprems)
-       apply (rule conjI; rule conjI; rule subprems)
-       apply (rule conjI; rule conjI; rule subprems)
+  apply (elim exE alt_ex1E conjE)
+  subgoal premises prems for z l r
+    apply (insert spec2[OF prems(1), of r z])
+    apply (insert spec2[OF prems(1), of l z])
+    apply (erule impE, intro conjI prems)
+    apply (erule impE, intro conjI prems)
+
     apply (rule exI)
     apply (unfold inf_fun_def inf_bool_def)
     apply (rule conjI)
-     apply (insert subprems) []
+     apply (insert prems) []
      apply (hypsubst_thin)
-    apply ((rule conjI)?,
+     apply ((rule conjI)?,
         rule subrelI, 
         rule CollectI, 
         rule case_prodI, 
         (rule conjI; erule rev_subsetD[THEN iffD1[OF prod_in_Collect_iff]]),
         assumption, assumption)+
-    apply (rule conjI)
-    apply (rule subprems)+
+    apply (rule conjI; rule prems)
     done
   done
 
-ML \<open>
-open BNF_Util BNF_Tactics
+(*
+lemma F_inj_map_strong2:
+  " (\<forall> R3 R4 Q3 Q4 (x :: ('a :: var,'b :: var,'c,'d) F) (y :: ('a :: var,'b :: var,'c,'d) F). rrel_F R3 R4 x y \<longrightarrow> rrel_F Q3 Q4 x y \<longrightarrow> rrel_F (inf R3 Q3) (inf R4 Q4) x y)
+  \<Longrightarrow> (\<And>p q.
+    p \<in> set3_F (x :: ('a :: var,'b :: var,'c,'d) F) \<Longrightarrow>
+    q \<in> set3_F (y :: ('a :: var,'b :: var,'c,'d) F) \<Longrightarrow> f1 p = g1 q \<Longrightarrow> f1' p = g1' q \<Longrightarrow> p = q)
+  \<Longrightarrow> (\<And>p q.
+    p \<in> set4_F x \<Longrightarrow>
+    q \<in> set4_F y \<Longrightarrow> f2 p = g2 q \<Longrightarrow> f2' p = g2' q \<Longrightarrow> p = q)
+  \<Longrightarrow> map_F id id f1 f2 x = map_F id id g1 g2 y 
+  \<Longrightarrow> map_F id id f1' f2' x = map_F id id g1' g2' y \<Longrightarrow> x = y"
+  subgoal premises prems
+    apply (insert prems(2, 3, 4, 5))
+    apply (drule F.rel_eq[THEN predicate2_eqD, THEN iffD2])
+    apply (drule F.rel_eq[THEN predicate2_eqD, THEN iffD2])
+    apply (rule F.rel_eq[THEN predicate2_eqD, THEN iffD1])
+    apply (drule F.rel_map(1)[THEN iffD1])
+    apply (drule F.rel_map(2)[THEN iffD1])
+    apply (drule F.rel_map(1)[THEN iffD1])
+    apply (drule F.rel_map(2)[THEN iffD1])
+    apply (drule prems(1)[rule_format]; assumption?)
+    apply (drule prems(1)[rule_format]; assumption?)
+    apply (unfold inf_bool_def inf_fun_def)
+    apply (erule F.rel_mono_strong)
+     apply (erule conjE)
+     apply (assumption)
+    apply (erule conjE)
+    apply (assumption)
+    done
+  done
 
-fun mk_rel_F_exchange_tac mrbnf F_mr_rel_mono_strong0 F_strong ctxt =
-  let
-    val id_prems = MRBNF_Comp_Tactics.mk_id_prems mrbnf;
-  in
-    HEADGOAL (Subgoal.FOCUS
-      (fn {prems, context = ctxt, ...} => 
-        HEADGOAL (EVERY' [
-          rtac ctxt (F_mr_rel_mono_strong0 OF flat (replicate 2 id_prems)),
-          rtac ctxt (F_strong OF prems),
-          K (unfold_thms_tac ctxt ([id_apply, eqTrueI OF [refl]] @ @{thms ball_triv inf_apply inf_bool_def}))
-        ]) THEN
-        ALLGOALS (
-          (rtac ctxt impI THEN' 
-          rtac ctxt TrueI) ORELSE'
-          (rtac ctxt ballI THEN' 
-          rtac ctxt ballI THEN'
-          rtac ctxt impI THEN'
-          eresolve_tac ctxt [conjunct1, conjunct2]))
-       ) ctxt)
-  end
-\<close>
+lemma spec6: "\<forall>x1 x2 x3 x4 x5 x6. P x1 x2 x3 x4 x5 x6 \<Longrightarrow> P x1 x2 x3 x4 x5 x6"
+  by blast
 
-(* lin_pos dependent? *)
+lemma "(\<forall> R3 R4 Q3 Q4 x y. rel_F id id R3 R4 (x :: ('a :: var,'b :: var,'c,'d) F) (y :: ('a :: var,'b :: var,'e,'f) F) \<longrightarrow> rel_F id id Q3 Q4 x y \<longrightarrow> rel_F id id (inf R3 Q3) (inf R4 Q4) x y)
+  \<longleftrightarrow>
+  (\<forall> R S (x :: ('a :: var,'b :: var,'c,'d) F) (y :: ('a :: var,'b :: var,'e,'f) F). (rrel_F R S x y =
+      (\<exists>!z. set3_F z \<subseteq> {(x, y). R x y} \<and>
+            set4_F z \<subseteq> {(x, y). S x y} \<and> map_F id id fst fst z = x \<and> map_F id id snd snd z = y)))"
+  apply (rule iffI)
+   prefer 2
+  apply (intro allI)
+  subgoal premises prem for R3 R4 Q3 Q4 x y
+    apply (intro impI)
+apply (frule F.mr_rel_mono_strong0[OF supp_id_bound bij_id supp_id_bound supp_id_bound bij_id supp_id_bound];
+      ((rule ballI, rule ballI refl)?, 
+        (rule impI, rule trans[OF top_apply[THEN fun_cong] trans[OF top_apply top_bool_def]])?)) 
+  apply (unfold F.map_id mr_rel_F_def eq_True)
+    apply (rotate_tac 2)
+  apply (drule prem[rule_format, THEN iffD1])
+  apply (unfold top_apply top_bool_def Collect_const_case_prod if_True eqTrueI[OF subset_UNIV] simp_thms(22))
+  apply (unfold F.in_rel[OF supp_id_bound bij_id supp_id_bound, unfolded id_apply F.map_id OO_Grp_alt]
+      id_def[symmetric] mem_Collect_eq)
+  apply (elim exE alt_ex1E conjE)
+    subgoal premises prems for z l r
+    apply (insert spec2[OF prems(1), of r z])
+    apply (insert spec2[OF prems(1), of l z])
+    apply (erule impE, intro conjI prems)
+    apply (erule impE, intro conjI prems)
+    apply (rule exI)
+    apply (unfold inf_fun_def inf_bool_def)
+    apply (rule conjI)
+     apply (insert prems) []
+     apply (hypsubst_thin)
+     apply ((rule conjI)?,
+        rule subrelI, 
+        rule CollectI, 
+        rule case_prodI, 
+        (rule conjI; erule rev_subsetD[THEN iffD1[OF prod_in_Collect_iff]]),
+        assumption, assumption)+
+    apply (rule conjI; rule prems)
+    done
+  done
+  apply (intro allI)
+  subgoal premises prem for R S x y
+    apply (auto)
+      apply (simp add: F.in_rel[OF supp_id_bound bij_id supp_id_bound, unfolded F.map_id])
+    thm prem[rule_format, unfolded mr_rel_F_def F.map_id]
+    subgoal for z y'
+      apply (hypsubst_thin)
+      thm spec6[OF prem, unfolded mr_rel_F_def F.map_id, rule_format] F_inj_map_strong2[rule_format]
+      sorry
+    subgoal for z
+      by (simp add: F.rel_map(1,2) F.rel_refl_strong subset_iff)
+    done
+  done
+thm F.inj_map_strong
+*)
+
 (* Another important consequence: the following "exchange"-property, which could be read: 
 Since the atoms have a fixed position, we can permute the relations: *)
 lemma rel_F_exchange: 
@@ -197,121 +223,32 @@ lemma rel_F_exchange:
   assumes "rel_F id id R3 R4 x x'" and "rel_F id id Q3 Q4 x x'"
   shows "rel_F id id R3 Q4 x x'" 
   using assms apply -
-  apply (tactic \<open>mk_rel_F_exchange_tac (MRBNF_Def.mrbnf_of @{context} @{type_name F} |> the) 
-    @{thm F.mr_rel_mono_strong0} @{thm F_strong} @{context} 
-    THEN print_tac @{context} "done" THEN no_tac\<close>)
   subgoal premises prems
     apply (rule F.mr_rel_mono_strong0[OF supp_id_bound bij_id supp_id_bound supp_id_bound bij_id supp_id_bound])
     apply (rule F_strong[OF prems])
        apply (unfold id_apply eqTrueI[OF refl] ball_triv inf_apply inf_bool_def)
        apply (intro impI TrueI)+
-     apply (intro ballI impI; erule conjunct1 conjunct2)+
+     apply (intro ballI impI; elim conjunct1 conjunct2)+
     done
   done
 
 (* Then notion of two items having the same shape (w.r.t. the 3rd position): *)
 (* these definitions are lin_pos dependent *)
-definition sameShape1 :: "('a1::var,'a2::var,'a3,'a4) F \<Rightarrow> ('a1,'a2,'a3,'a4) F \<Rightarrow> bool" where 
-  "sameShape1 x x' \<equiv> rel_F id id top (=) x x'"
+definition sameShape :: "('a1::var,'a2::var,'a3,'a4) F \<Rightarrow> ('a1,'a2,'a3,'a4) F \<Rightarrow> bool" where 
+  "sameShape x x' \<equiv> rel_F id id top (=) x x'"
 
-definition nonrep2 :: "('a1::var,'a2::var,'a3,'a4) F \<Rightarrow> bool" where 
-  "nonrep2 x \<equiv> \<forall> x'. sameShape1 x x' \<longrightarrow> (\<exists> f. x' = map_F id id f id x)"
+definition nonrep :: "('a1::var,'a2::var,'a3,'a4) F \<Rightarrow> bool" where 
+  "nonrep x \<equiv> \<forall> x'. sameShape x x' \<longrightarrow> (\<exists> f. x' = map_F id id f id x)"
 
-ML\<open>
-open BNF_Util BNF_Tactics
-
-fun mk_nonrep2_map_F_tac mrbnf nonrep_def sameShape_def F_map_comp F_mr_rel_map mr_rel_F_def F_rel_compp 
-  F_rel_Grp F_map_id F_in_rel F_rel_maps F_rel_refl_strong ctxt = 
-  HEADGOAL (Subgoal.FOCUS 
-    (fn {prems, context = ctxt, ...} => 
-      let
-        val var_types = var_types_of_mrbnf mrbnf;
-        val nr_lives = length (filter (fn v => v = MRBNF_Def.Live_Var) var_types);
-        val nr_non_lives = length (filter (fn v => not (v = MRBNF_Def.Live_Var)) var_types);
-        val lin_live_pos = fold_index (fn (i, v) => fn b => 
-          if (v = MRBNF_Def.Live_Var andalso i+1 < lin_pos) then b+1 else b) var_types 1;
-        val switch_poses = map_range (fn i => if i < (lin_pos-(lin_live_pos)) then i+1 else i+2) (nr_non_lives);
-        val switch = (fn thm1 => (fn thm2 => trans OF [thm1, thm2 RS sym]));
-        val o_id = @{thm o_id};
-        val id_o = @{thm id_o};
-      in
-        unfold_thms_tac ctxt [nonrep_def, sameShape_def] THEN
-        HEADGOAL (EVERY' [
-          rtac ctxt allI,
-          rtac ctxt impI,
-          etac ctxt exE,
-          EqSubst.eqsubst_tac ctxt [0] [F_map_comp] THEN_ALL_NEW
-            TRY o resolve_tac ctxt (prems @ @{thms supp_id_bound bij_id}),
-          K (unfold_thms_tac ctxt [switch id_o o_id]),
-          EqSubst.eqsubst_tac ctxt [lin_pos] [switch o_id id_o], (*move all id to the right except for lin_pos*)
-          EqSubst.eqsubst_tac ctxt [0] [F_map_comp RS sym] THEN_ALL_NEW
-            TRY o resolve_tac ctxt (prems @ @{thms supp_id_bound bij_id}),
-          dtac ctxt (rotate_prems ~1 (F_mr_rel_map RS iffD1)) THEN_ALL_NEW
-            TRY o resolve_tac ctxt (prems @ @{thms supp_id_bound bij_id}),
-          K (unfold_thms_tac ctxt [switch id_o o_id, @{thm Grp_UNIV_id}]),
-          K (unfold_thms_tac ctxt [switch @{thm OO_eq} @{thm eq_OO}]),  
-          EqSubst.eqsubst_asm_tac ctxt [lin_live_pos] [switch @{thm eq_OO} @{thm OO_eq}], (*move all (=) to the left except for lin_live_pos*)
-          K (unfold_thms_tac ctxt @{thms eq_alt}),   
-          EqSubst.eqsubst_tac ctxt [0] @{thms Grp_UNIV_id}
-        ]) THEN
-        unfold_thms_tac ctxt [mr_rel_F_def, o_id, F_rel_compp, F_rel_Grp] THEN
-        unfold_thms_tac ctxt [eqTrueI OF @{thms subset_UNIV}, @{thm simp_thms(21)}, id_o, @{thm UNIV_def} RS sym] THEN
-        unfold_thms_tac ctxt ([eqTrueI OF [@{thm UNIV_I}], id_apply] @ @{thms Grp_UNIV_id OO_def Grp_def simp_thms(21)}) THEN
-        HEADGOAL (EVERY' [
-          etac ctxt exE,
-          etac ctxt conjE,
-          dtac ctxt (rotate_prems ~1 (F_in_rel RS iffD1)) THEN_ALL_NEW
-            TRY o resolve_tac ctxt prems,
-          Method.insert_tac ctxt [unfold_thms ctxt [nonrep_def, sameShape_def, mr_rel_F_def, F_map_id] 
-            (nth prems (length prems -1))],
-          etac ctxt exE,
-          etac ctxt conjE,
-          etac ctxt CollectE,
-          etac ctxt conjE
-        ]) THEN
-        REPEAT_DETERM_N (nr_lives-1) (HEADGOAL (
-          etac ctxt conjE)) THEN
-        HEADGOAL (hyp_subst_tac_thin true ctxt) THEN
-        HEADGOAL (Subgoal.FOCUS 
-          (fn {prems = subprems, context = ctxt, params, ...} => 
-            HEADGOAL (EVERY' [
-              Method.insert_tac ctxt [nth subprems 0],
-              etac ctxt allE,
-              etac ctxt impE,
-              rtac ctxt (infer_instantiate' ctxt [NONE, SOME (snd (nth params 1))] exI),
-              EqSubst.eqsubst_tac ctxt [1] [nth F_rel_maps 0],
-              EqSubst.eqsubst_tac ctxt [1] [nth F_rel_maps 1]
-            ]) THEN
-            HEADGOAL (rtac ctxt F_rel_refl_strong) THEN
-            REPEAT_DETERM_N nr_lives (HEADGOAL (
-                (dresolve_tac ctxt (map (fn p => subsetD OF [p] RS @{thm Collect_case_prodD}) (drop 1 subprems)) THEN'
-                  (assume_tac ctxt ORELSE' 
-                  (rtac ctxt sym THEN' assume_tac ctxt))))) THEN
-            HEADGOAL (EVERY' [
-              etac ctxt exE,
-              EqSubst.eqsubst_tac ctxt [0] [F_map_comp] THEN_ALL_NEW
-                TRY o resolve_tac ctxt (prems @ @{thms supp_id_bound bij_id}),
-              EqSubst.eqsubst_tac ctxt switch_poses [switch id_o o_id],
-              EqSubst.eqsubst_tac ctxt [0] [F_map_comp RS sym] THEN_ALL_NEW
-                TRY o resolve_tac ctxt (prems @ @{thms supp_id_bound bij_id}),
-              rtac ctxt exI,
-              dtac ctxt arg_cong,
-              assume_tac ctxt
-            ]) 
-          ) ctxt)
-      end)
-  ctxt)
-\<close>
-
-lemma nonrep2_map_F:
+lemma nonrep_map_F:
   fixes x :: "('a1::var,'a2::var,'a3,'a4) F"
     and v :: "'a1 \<Rightarrow> 'a1" and u :: "'a2\<Rightarrow>'a2" and g :: "'a4 \<Rightarrow> 'b4"
   assumes v: "|supp v| <o |UNIV :: 'a1 set|"  and u: "bij u" "|supp u| <o |UNIV :: 'a2 set|" 
-  assumes "nonrep2 x"
-  shows "nonrep2 (map_F v u id g x)"
+  assumes "nonrep x"
+  shows "nonrep (map_F v u id g x)"
   using assms apply -
   subgoal premises prems
-    apply (unfold nonrep2_def sameShape1_def)
+    apply (unfold nonrep_def sameShape_def)
     apply (rule allI)
     apply (rule impI)
     apply (subst F.map_comp; (rule prems bij_id supp_id_bound)?)
@@ -333,7 +270,7 @@ lemma nonrep2_map_F:
     apply (erule CollectE)
     apply (erule conjE)
     apply (erule conjE)
-    apply (insert prems(4)[unfolded nonrep2_def sameShape1_def mr_rel_F_def F.map_id])
+    apply (insert prems(4)[unfolded nonrep_def sameShape_def mr_rel_F_def F.map_id])
     apply (rotate_tac -1)
     apply (hypsubst_thin)
     subgoal premises subprems for x' y z
@@ -350,7 +287,7 @@ lemma nonrep2_map_F:
       apply (subst F.map_comp[OF _ _ _ supp_id_bound bij_id supp_id_bound, unfolded trans[OF id_o o_id[symmetric]]]; (rule prems)?)
       apply (subst F.map_comp[THEN sym]; (rule prems bij_id supp_id_bound)?)
       subgoal premises subprems for f
-        apply (rule exI[of _ f]) (* instantiation not necessary but easy*)
+        apply (rule exI[of _ f])
         apply (subst subprems)
         apply (subst F.map_comp; (rule prems bij_id supp_id_bound)?)
         apply (unfold o_id id_o)
@@ -360,223 +297,65 @@ lemma nonrep2_map_F:
     done
   done
 
-ML\<open>
-open BNF_Util BNF_Tactics
-
-fun mk_nonrep2_map_F_rev_tac mrbnf nonrep_def sameShape_def F_mr_rel_map1 F_mr_rel_map2 F_mr_rel_map3 F_map_comp F_rel_eq 
-  F_mr_rel_id rel_F_exchange F_mr_rel_flip F_mr_rel_mono_strong0 F_mr_rel_Grp ctxt = 
-  HEADGOAL (Subgoal.FOCUS 
-    (fn {prems, context = ctxt, ...} => 
-      let
-        val var_types = var_types_of_mrbnf mrbnf;
-        val nr_lives = length (filter (fn v => v = MRBNF_Def.Live_Var) var_types);
-        val nr_non_lives = length (filter (fn v => not (v = MRBNF_Def.Live_Var)) var_types);
-        val lin_live_pos = fold_index (fn (i, v) => fn b => 
-          if (v = MRBNF_Def.Live_Var andalso i+1 < lin_pos) then b+1 else b) var_types 1;
-        val switch = (fn thm1 => (fn thm2 => trans OF [thm1, thm2 RS sym]));
-      in
-        unfold_thms_tac ctxt [nonrep_def, sameShape_def] THEN
-        HEADGOAL (EVERY' [
-          rtac ctxt allI,
-          rtac ctxt impI,
-          etac ctxt exE,
-          forward_tac ctxt [rotate_prems ~1 F_mr_rel_map2] THEN_ALL_NEW
-            TRY o resolve_tac ctxt (prems @ @{thms supp_id_bound bij_id}),
-          rotate_tac 1,
-          EqSubst.eqsubst_asm_tac ctxt (map_range (fn i => i+1) nr_non_lives) [switch @{thm o_id} @{thm id_o}],
-          EqSubst.eqsubst_asm_tac ctxt [lin_live_pos] @{thms Grp_UNIV_id},
-          K (unfold_thms_tac ctxt [switch @{thm eq_OO} @{thm OO_eq}]),
-          EqSubst.eqsubst_asm_tac ctxt [lin_live_pos] [switch @{thm OO_eq} @{thm eq_OO}], (*move all (=) to the right and then lin_live_pos back*)
-          EqSubst.eqsubst_asm_tac ctxt [lin_live_pos] @{thms eq_alt},
-          EqSubst.eqsubst_asm_tac ctxt [0] [F_mr_rel_map1 RS sym] THEN_ALL_NEW
-            TRY o resolve_tac ctxt (prems @ @{thms supp_id_bound bij_id}),
-          Method.insert_tac ctxt [unfold_thms ctxt [nonrep_def, sameShape_def] (nth prems (length prems - 1))],
-          etac ctxt allE,
-          etac ctxt impE,
-          rtac ctxt exI,
-          assume_tac ctxt,
-          etac ctxt thin_rl,
-          etac ctxt exE,
-          EqSubst.eqsubst_asm_tac ctxt [0] [F_map_comp] THEN_ALL_NEW
-            TRY o resolve_tac ctxt (prems @ @{thms supp_id_bound bij_id}),
-          K (unfold_thms_tac ctxt @{thms id_o o_id}),
-          EqSubst.eqsubst_asm_tac ctxt [1] [F_rel_eq RS sym],
-          EqSubst.eqsubst_asm_tac ctxt [1] [F_mr_rel_id],
-          dtac ctxt (rotate_prems ~1 (iffD1 OF [F_mr_rel_map1])) THEN_ALL_NEW
-            TRY o resolve_tac ctxt (prems @ @{thms supp_id_bound bij_id}),
-          K (unfold_thms_tac ctxt @{thms id_o OO_eq}),
-          dtac ctxt (rotate_prems 1 rel_F_exchange),
-          rtac ctxt (F_mr_rel_flip RS iffD1) THEN_ALL_NEW
-            TRY o resolve_tac ctxt @{thms supp_id_bound bij_id},
-          K (unfold_thms_tac ctxt @{thms inv_id}),
-          EqSubst.eqsubst_asm_tac ctxt [0] [F_mr_rel_map3] THEN_ALL_NEW
-            TRY o resolve_tac ctxt (prems @ @{thms supp_id_bound bij_id}),
-          EqSubst.eqsubst_asm_tac ctxt (map_range (fn i => i+1) (2 * nr_lives)) @{thms Grp_def},
-          EqSubst.eqsubst_asm_tac ctxt (map_range (fn i => i+1) (nr_non_lives)) @{thms inv_o_simp1} THEN_ALL_NEW
-            TRY o resolve_tac ctxt (@{thm bij_id}::prems),
-          K (unfold_thms_tac ctxt ((eqTrueI OF @{thms UNIV_I}):: @{thms id_apply simp_thms(21)})),
-          EqSubst.eqsubst_asm_tac ctxt [lin_live_pos] @{thms eq_commute},
-          K (unfold_thms_tac ctxt @{thms eq_OO conversep_def}),
-          etac ctxt (rotate_prems (~1 - (length var_types)) F_mr_rel_mono_strong0) THEN_ALL_NEW
-            TRY o resolve_tac ctxt @{thms supp_id_bound bij_id}
-        ]) THEN
-        REPEAT_DETERM_N (length var_types) (
-          (HEADGOAL (
-            (* for bound and free *)
-            rtac ctxt ballI THEN'
-            rtac ctxt refl)) 
-          ORELSE 
-          (HEADGOAL (
-            (* for lives*)
-            rtac ctxt ballI THEN'
-            rtac ctxt ballI THEN'
-            rtac ctxt impI THEN'
-            rotate_tac 2 THEN'
-            EqSubst.eqsubst_asm_tac ctxt [0] @{thms eq_commute} THEN'
-            assume_tac ctxt))
-        ) THEN
-        HEADGOAL (EVERY' [
-          etac ctxt thin_rl,
-          EqSubst.eqsubst_asm_tac ctxt [lin_live_pos] [@{thm Grp_UNIV_def} RS sym],
-          rtac ctxt exI,
-          EqSubst.eqsubst_asm_tac ctxt (map_range (fn i => i+1) (nr_lives -1)) @{thms eq_alt},
-          EqSubst.eqsubst_asm_tac ctxt [0] [F_mr_rel_Grp] THEN_ALL_NEW
-            TRY o resolve_tac ctxt @{thms supp_id_bound bij_id}
-        ]) THEN
-        unfold_thms_tac ctxt ([eqTrueI OF @{thms subset_UNIV}, eqTrueI OF @{thms UNIV_I}, @{thm UNIV_def} RS sym] @ 
-          @{thms simp_thms(21) Grp_def}) THEN
-        HEADGOAL (assume_tac ctxt)
-      end)
-  ctxt)
-\<close>
-
 (* Here we need pullback preservation: *)
-lemma nonrep2_map_F_rev:
+lemma nonrep_map_F_rev:
   fixes x :: "('a1::var,'a2::var,'a3,'a4) F" and u :: "'a2\<Rightarrow>'a2" and g :: "'a4 \<Rightarrow> 'a4'"
   assumes u: "bij u" "|supp u| <o |UNIV :: 'a2 set|" 
-  assumes "nonrep2 (map_F id u id g x)"
-  shows "nonrep2 x"
+  assumes "nonrep (map_F id u id g x)"
+  shows "nonrep x"
   using assms apply -
- (* apply (tactic \<open>mk_nonrep2_map_F_rev_tac (MRBNF_Def.mrbnf_of @{context} @{type_name F} |> the) @{thm nonrep2_def} @{thm sameShape1_def} @{thm F.mr_rel_map(1)}
-    @{thm F.mr_rel_map(2)} @{thm F.mr_rel_map(3)} @{thm F.map_comp} @{thm F.rel_eq} @{thm F.mr_rel_id} @{thm rel_F_exchange} 
-    @{thm F.mr_rel_flip} @{thm F.mr_rel_mono_strong0} @{thm F.mr_rel_Grp} @{context} 
-    THEN print_tac @{context} "done" THEN no_tac\<close>)*)
   subgoal premises prems
-    apply (unfold nonrep2_def sameShape1_def)
+    apply (unfold nonrep_def sameShape_def)
     apply (rule allI)
     apply (rule impI)
-
-(* alt *)
-    apply (insert prems(3)[unfolded nonrep2_def sameShape1_def]) (*lastprem*)
+    apply (insert prems(3)[unfolded nonrep_def sameShape_def])
     apply (elim allE impE)
      apply (rule F.mr_rel_map(1)[THEN iffD2]; (rule prems supp_id_bound bij_id)?)
-  (*_ * (2*nr_BF + nr_As + 2(x,y)) *)
    apply (drule F.mr_rel_map(2)[rotated -1, of _ _ _ _ _ _ _ _ id _]; (rule prems supp_id_bound bij_id)?)
      apply (unfold o_id id_o Grp_UNIV_id eq_OO OO_eq)
      apply (assumption)
-(*
-    apply (rotate_tac)
-    apply (subst (asm) (1 2) trans[OF o_id id_o[symmetric]]) (*1..nr_non_lives*)
-    apply (subst (asm) (1) Grp_UNIV_id) (*lin_live_pos*)
-    apply (unfold trans[OF eq_OO OO_eq[symmetric]])
-    apply (subst (asm) (1) trans[OF OO_eq eq_OO[symmetric]]) (*lin_live_pos*)
-    apply (subst (asm) (1) eq_alt) (*lin_live_pos*)
-    thm eq_alt Grp_UNIV_id trans[OF OO_eq eq_OO[symmetric]]
-    apply (subst (asm) F.mr_rel_map(1)[symmetric]; (rule prems supp_id_bound bij_id)?)
-     apply (assumption)
-*)
-
     apply (erule exE)
     apply (subst (asm) F.map_comp; (rule prems supp_id_bound bij_id)?)
     apply (unfold o_id id_o)
-
-    thm F.map_cong
-
     apply (subst (asm) F.rel_eq[symmetric])
     apply (unfold F.mr_rel_id)
-    thm F.mr_rel_map
     apply (drule iffD1[OF F.mr_rel_map(1), rotated -1]; (rule prems supp_id_bound bij_id)?)
     apply (unfold id_o OO_eq)
-    thm rel_F_exchange[rotated]
     apply (drule rel_F_exchange[rotated])
      apply (rule iffD1[OF F.mr_rel_flip]; (rule supp_id_bound bij_id)?)
     apply (unfold inv_id)
      apply (subst (asm) F.mr_rel_map(3); (rule prems supp_id_bound bij_id)?)
-     apply ((*subst (asm) (1 2 3 4)*) unfold Grp_def) (*TWICE for all lives *)
-    apply (subst (asm) (1 2) inv_o_simp1; (rule prems bij_id)?) (*for all frees and bounds*)
-     apply (tactic \<open>unfold_thms_tac @{context} @{thms eqTrueI[OF UNIV_I] simp_thms(21) id_apply}\<close>) (*for all frees*)
-     apply (subst (asm) (1) eq_commute) (*lin_live_pos*)
+     apply (unfold Grp_def)
+    apply (subst (asm) (1 2) inv_o_simp1; (rule prems bij_id)?)
+     apply (tactic \<open>Ctr_Sugar_Tactics.unfold_thms_tac @{context} @{thms eqTrueI[OF UNIV_I] simp_thms(21) id_apply}\<close>)
+     apply (subst (asm) eq_commute)
      apply (unfold eq_OO conversep_def)
-     apply (elim F.mr_rel_mono_strong0[rotated -5]; (rule supp_id_bound bij_id)?) (*- len vartypes - 1*)
+     apply (elim F.mr_rel_mono_strong0[rotated -5]; (rule supp_id_bound bij_id)?)
       (*left subtactic is for frees and bounds, right subtactic for lives*)
     apply ((rule ballI,rule refl)?; (rule ballI,rule ballI,rule impI,rotate_tac 2,subst (asm) eq_commute,assumption))+
 
     apply (erule thin_rl)
-    apply (subst (asm) (1) Grp_UNIV_def[symmetric]) (*lin_live_pos*)
+    apply (subst (asm) Grp_UNIV_def[symmetric])
     apply (rule exI)
-    apply (subst (asm) (1) eq_alt) (* repeat lives - 1 *)
-    thm F.mr_rel_Grp
+    apply (subst (asm) eq_alt)
     apply (subst (asm) F.mr_rel_Grp; (rule supp_id_bound bij_id)?)
     apply (unfold eqTrueI[OF subset_UNIV] eqTrueI[OF UNIV_I] UNIV_def[THEN sym] simp_thms(21) Grp_def)
     apply (assumption)
     done
   done
 
-ML\<open>
-open BNF_Util BNF_Tactics
-fun mk_nonrep2_map_bij_tac nonrep_def sameShape_def F_mr_rel_map1 F_map_comp cgs ctxt = 
-  HEADGOAL (Subgoal.FOCUS 
-    (fn {prems, context = ctxt, ...} => 
-      unfold_thms_tac ctxt [nonrep_def, sameShape_def] THEN
-      HEADGOAL (EVERY' [
-        rtac ctxt allI,
-        rtac ctxt impI,
-        dtac ctxt (rotate_prems ~1 (F_mr_rel_map1 RS iffD1)) THEN_ALL_NEW
-          TRY o resolve_tac ctxt @{thms bij_id supp_id_bound},
-        K (unfold_thms_tac ctxt @{thms o_id Grp_UNIV_id eq_OO Grp_OO_top}),
-        dtac ctxt (Object_Logic.rulify ctxt (unfold_thms ctxt [nonrep_def, sameShape_def] (nth prems 1))),
-        etac ctxt exE,
-        hyp_subst_tac_thin true ctxt
-      ]) THEN
-      unfold_thms_tac ctxt @{thms triv_forall_equality} THEN
-      HEADGOAL (Subgoal.FOCUS 
-        (fn {context = ctxt, params, ...} => 
-          HEADGOAL (EVERY' (map (fn ((_, cf), cg) => 
-            let
-              val g = Thm.term_of cg
-              val (dom_g, rng_g) = fastype_of g |> dest_funT
-              val inv_g = Const ("Hilbert_Choice.inv", 
-                (fastype_of g) --> (rng_g --> dom_g)) $ g
-              val f_o_inv_g = HOLogic.mk_comp (Thm.term_of cf, inv_g)
-            in
-              rtac ctxt (infer_instantiate' ctxt [NONE, SOME (Thm.cterm_of ctxt f_o_inv_g)] exI) 
-            end) (params ~~ cgs))
-          ) THEN
-          HEADGOAL (rtac ctxt sym) THEN
-          HEADGOAL (rtac ctxt trans) THEN
-          HEADGOAL (rtac ctxt F_map_comp THEN_ALL_NEW
-            TRY o resolve_tac ctxt @{thms bij_id supp_id_bound}) THEN
-          unfold_thms_tac ctxt ([@{thm inv_o_simp1} OF (take 1 prems), @{thm o_assoc} RS sym] @ @{thms id_o o_id}) THEN
-          HEADGOAL (rtac ctxt refl)
-        ) ctxt)
-  ) ctxt)
-\<close>
-
-lemma nonrep2_mapF_bij:
+lemma nonrep_mapF_bij:
   fixes x :: "('a1::var,'a2::var,'a3,'a4) F" and g::"'a3\<Rightarrow>'a3"
-  assumes g: "bij g" and x: "nonrep2 x"
-  shows "nonrep2 (map_F id id g id x)" (is "nonrep2 ?x'")
+  assumes g: "bij g" and x: "nonrep x"
+  shows "nonrep (map_F id id g id x)" (is "nonrep ?x'")
   using assms apply -
-  apply (tactic \<open>mk_nonrep2_map_bij_tac @{thm nonrep2_def}
-    @{thm sameShape1_def} @{thm F.mr_rel_map(1)} @{thm F.map_comp} [@{cterm g}] @{context}
-    THEN print_tac @{context} "done" THEN no_tac\<close>) 
   subgoal premises prems
-    apply (unfold nonrep2_def sameShape1_def)
+    apply (unfold nonrep_def sameShape_def)
     apply (rule allI)
     apply (rule impI)
     apply (drule F.mr_rel_map(1)[THEN iffD1, rotated -1]; (rule supp_id_bound bij_id)?)
     apply (unfold o_id Grp_UNIV_id eq_OO Grp_OO_top)
-    apply (drule x[unfolded nonrep2_def sameShape1_def, rule_format])
+    apply (drule x[unfolded nonrep_def sameShape_def, rule_format])
     apply (erule exE conjE)+
     apply hypsubst_thin
     subgoal for _ f
@@ -590,40 +369,21 @@ lemma nonrep2_mapF_bij:
     done
   done
 
-ML \<open>
-open BNF_Util BNF_Tactics
-
-fun mk_nonrep2_mapF_bij_2_tac mrbnf nonrep2_mapF_bij nonrep2_map_F F_map_comp ctxt =
-  HEADGOAL (Subgoal.FOCUS
-    (fn {prems, context = ctxt, ...} => 
-    let val nr_prems = length prems;
-        val id_prems = MRBNF_Comp_Tactics.mk_id_prems mrbnf;
-    in
-      HEADGOAL (rtac ctxt (unfold_thms ctxt ((F_map_comp OF ((take (nr_prems-2) prems) @ id_prems)) :: @{thms id_o o_id}) 
-        (nonrep2_mapF_bij OF [nth prems (nr_prems-2), nonrep2_map_F OF (nth_drop (nr_prems-2) prems)])
-      ))
-     end) ctxt)
-\<close>
-
-lemma nonrep2_mapF_bij_2:
+lemma nonrep_mapF_bij_2:
   fixes x :: "('a1::var,'a2::var,'a3,'a4) F"
     and v :: "'a1 \<Rightarrow> 'a1" and u :: "'a2\<Rightarrow>'a2" and g::"'a3\<Rightarrow>'a3" and f::"'a4\<Rightarrow>'a4'"
   assumes v: "|supp v| <o |UNIV :: 'a1 set|" and u: "bij u" "|supp u| <o |UNIV :: 'a2 set|"
-    and g: "bij g" and x: "nonrep2 x"
-  shows "nonrep2 (map_F v u g f x)" 
+    and g: "bij g" and x: "nonrep x"
+  shows "nonrep (map_F v u g f x)" 
   using assms apply -
-  apply (tactic \<open>mk_nonrep2_mapF_bij_2_tac (MRBNF_Def.mrbnf_of @{context} @{type_name F} |> the) 
-    @{thm nonrep2_mapF_bij} @{thm nonrep2_map_F} @{thm F.map_comp} @{context} 
-    THEN print_tac @{context} "done" THEN no_tac\<close>)
   subgoal premises prems
-    apply (rule nonrep2_mapF_bij[OF prems(4) nonrep2_map_F[OF prems(1,2,3,5)], 
+    apply (rule nonrep_mapF_bij[OF prems(4) nonrep_map_F[OF prems(1,2,3,5)], 
           unfolded F.map_comp[OF prems(1,2,3) supp_id_bound bij_id supp_id_bound] id_o o_id])
     done
   done
 
-
-typedef ('a1::var,'a2::var,'a3::var,'a4) F' = "{x :: ('a1,'a2,'a3,'a4) F. nonrep2 x}"
-  apply (unfold mem_Collect_eq nonrep2_def sameShape1_def mr_rel_F_def F.map_id)
+typedef ('a1::var,'a2::var,'a3::var,'a4) F' = "{x :: ('a1,'a2,'a3,'a4) F. nonrep x}"
+  apply (unfold mem_Collect_eq nonrep_def sameShape_def mr_rel_F_def F.map_id)
   by (rule ex_nonrep)
 
 definition set1_F' :: "('a1::var,'a2::var,'a3::var,'a4) F' \<Rightarrow> 'a1 set" where "set1_F' = set1_F o Rep_F'"
@@ -670,7 +430,7 @@ lemma F'_map_comp1_:
     apply (subst F.map_comp0; (rule prems)?)
     apply (unfold o_apply)
     apply (subst Abs_F'_inverse[unfolded mem_Collect_eq])
-     apply (rule nonrep2_mapF_bij_2; (rule prems Rep_F'[unfolded mem_Collect_eq])?)
+     apply (rule nonrep_mapF_bij_2; (rule prems Rep_F'[unfolded mem_Collect_eq])?)
     apply (rule refl)
     done
   done
@@ -680,13 +440,13 @@ lemma F'_map_comp1_:
 ML \<open>
 open BNF_Util BNF_Tactics
 
-fun mk_set_map_tac set_F'_def map_F'_def Abs_F'_inverse Rep_F' nonrep2_mapF_bij_2 F_set_map ctxt =
+fun mk_set_map_tac set_F'_def map_F'_def Abs_F'_inverse Rep_F' nonrep_mapF_bij_2 F_set_map ctxt =
   HEADGOAL (Subgoal.FOCUS
     (fn {prems = prems, context = ctxt, ...} =>
       unfold_thms_tac ctxt ([set_F'_def, map_F'_def] @ map (fn thm => thm RS eqTrueI) prems @
         @{thms asSS_def asBij_def if_True o_apply}) THEN
       HEADGOAL (EVERY' [EqSubst.eqsubst_tac ctxt [0] [Abs_F'_inverse],
-        rtac ctxt nonrep2_mapF_bij_2 THEN_ALL_NEW resolve_tac ctxt (Rep_F' :: prems),
+        rtac ctxt nonrep_mapF_bij_2 THEN_ALL_NEW resolve_tac ctxt (Rep_F' :: prems),
         rtac ctxt F_set_map THEN_ALL_NEW
           resolve_tac ctxt prems])
     ) ctxt)
@@ -701,14 +461,14 @@ lemma F'_set1_map_:
   assumes "bij u3" "|supp u3| <o |UNIV :: 'a3 set|"
   shows "set1_F' (map_F' u1 u2 u3 f b) = u1 ` set1_F' b"
   using assms apply -
-  apply (tactic \<open>mk_set_map_tac @{thm set1_F'_def} @{thm map_F'_def} @{thm Abs_F'_inverse[unfolded mem_Collect_eq]}
-    @{thm Rep_F'[unfolded mem_Collect_eq]} @{thm nonrep2_mapF_bij_2} @{thm F.set_map(1)} @{context} 
-    THEN print_tac @{context} "done" THEN no_tac\<close>)
+ (* apply (tactic \<open>mk_set_map_tac @{thm set1_F'_def} @{thm map_F'_def} @{thm Abs_F'_inverse[unfolded mem_Collect_eq]}
+    @{thm Rep_F'[unfolded mem_Collect_eq]} @{thm nonrep_mapF_bij_2} @{thm F.set_map(1)} @{context} 
+    THEN print_tac @{context} "done" THEN no_tac\<close>)*)
   subgoal premises prems
     apply (unfold set1_F'_def map_F'_def asSS_def asBij_def
         eqTrueI[OF prems(1)] eqTrueI[OF prems(2)] eqTrueI[OF prems(3)] eqTrueI[OF prems(4)] eqTrueI[OF prems(5)] o_apply if_True)
     apply (subst Abs_F'_inverse[unfolded mem_Collect_eq])
-     apply (rule nonrep2_mapF_bij_2; (rule prems Rep_F'[unfolded mem_Collect_eq])?)
+     apply (rule nonrep_mapF_bij_2; (rule prems Rep_F'[unfolded mem_Collect_eq])?)
     apply (rule F.set_map(1); (rule prems))
     done
   done
@@ -723,7 +483,7 @@ lemma F'_set2_map_:
   shows "set2_F' (map_F' u1 u2 u3 f b) = u2 ` set2_F' b"
   using assms apply -
   apply (tactic \<open>mk_set_map_tac @{thm set2_F'_def} @{thm map_F'_def} @{thm Abs_F'_inverse[unfolded mem_Collect_eq]}
-    @{thm Rep_F'[unfolded mem_Collect_eq]} @{thm nonrep2_mapF_bij_2} @{thm F.set_map(2)} @{context}\<close>)
+    @{thm Rep_F'[unfolded mem_Collect_eq]} @{thm nonrep_mapF_bij_2} @{thm F.set_map(2)} @{context}\<close>)
   done
 
 lemma F'_set3_map_:
@@ -736,7 +496,7 @@ lemma F'_set3_map_:
   shows "set3_F' (map_F' u1 u2 u3 f b) = u3 ` set3_F' b"
   using assms apply -
   apply (tactic \<open>mk_set_map_tac @{thm set3_F'_def} @{thm map_F'_def} @{thm Abs_F'_inverse[unfolded mem_Collect_eq]}
-    @{thm Rep_F'[unfolded mem_Collect_eq]} @{thm nonrep2_mapF_bij_2} @{thm F.set_map(3)} @{context}\<close>)
+    @{thm Rep_F'[unfolded mem_Collect_eq]} @{thm nonrep_mapF_bij_2} @{thm F.set_map(3)} @{context}\<close>)
   done
 
 lemma F'_set4_map_:
@@ -749,7 +509,7 @@ lemma F'_set4_map_:
   shows "set4_F' (map_F' u1 u2 u3 f b) = f ` set4_F' b"
   using assms apply -
   apply (tactic \<open>mk_set_map_tac @{thm set4_F'_def} @{thm map_F'_def} @{thm Abs_F'_inverse[unfolded mem_Collect_eq]}
-    @{thm Rep_F'[unfolded mem_Collect_eq]} @{thm nonrep2_mapF_bij_2} @{thm F.set_map(4)} @{context}\<close>)
+    @{thm Rep_F'[unfolded mem_Collect_eq]} @{thm nonrep_mapF_bij_2} @{thm F.set_map(4)} @{context}\<close>)
   done
 
 lemma F'_map_cong_[fundef_cong]:
@@ -833,7 +593,7 @@ lemma F'_in_rel:
         eqTrueI[OF prems(5)]
         eqTrueI[OF supp_id_bound] eqTrueI[OF bij_id] o_apply)
     apply (subst Abs_F'_inverse[unfolded mem_Collect_eq])
-     apply (rule nonrep2_mapF_bij_2; (rule prems Rep_F'[unfolded mem_Collect_eq])?)
+     apply (rule nonrep_mapF_bij_2; (rule prems Rep_F'[unfolded mem_Collect_eq])?)
 
 (* instantiation for bounds B, frees F, lives A: [_ * nr_BFs @ id * nr_BFs @ _ * nr_As @ id * nr_As] *)
     apply (subst F.map_comp[of _ _ id id _ _ id id, unfolded o_id id_o, symmetric]; (rule prems bij_id supp_id_bound)?)
@@ -852,7 +612,7 @@ lemma F'_in_rel:
       apply ((subst Abs_F'_inverse[unfolded mem_Collect_eq]), (tactic \<open>defer_tac 1\<close>))+ 
          apply (tactic \<open>distinct_subgoals_tac\<close>)
       prefer 2
-       apply (rule nonrep2_map_F_rev; (rule bij_id supp_id_bound)?)
+       apply (rule nonrep_map_F_rev; (rule bij_id supp_id_bound)?)
        apply (subst F.map_comp; (rule bij_id supp_id_bound)?)
        apply (unfold o_id id_o)
        apply (subst subprems)
@@ -885,13 +645,13 @@ lemma F'_in_rel:
     subgoal premises subprems for z
       apply (rule exI)
       apply (subst Abs_F'_inverse[unfolded mem_Collect_eq])
-       apply (rule nonrep2_mapF_bij_2; (rule supp_id_bound bij_id Rep_F'[unfolded mem_Collect_eq])?)
+       apply (rule nonrep_mapF_bij_2; (rule supp_id_bound bij_id Rep_F'[unfolded mem_Collect_eq])?)
       apply (rule conjI; (rule conjI)?)
 
         prefer 3(* subgoal 3 is solvable without the exI instantiation and it "instantiates" ?z 
           so that the other 2 subgoals are solvable as well*)
         apply (subst Abs_F'_inverse[unfolded mem_Collect_eq])
-         apply (rule nonrep2_mapF_bij_2; (rule prems Rep_F'[unfolded mem_Collect_eq])?)
+         apply (rule nonrep_mapF_bij_2; (rule prems Rep_F'[unfolded mem_Collect_eq])?)
         apply (subst F.map_comp; (rule bij_id supp_id_bound prems)?) (*having the id prems before the actual prems is important!*)
         apply (unfold o_id)
         apply (unfold o_def)
@@ -920,22 +680,7 @@ lemma F'_in_rel:
     done
   done
 
-ML \<open>
-open BNF_Util BNF_Tactics
-
-fun mk_strong_tac rrel_F'_def mr_rel_F_def F_strong F_map_id ctxt =
-  HEADGOAL (Subgoal.FOCUS
-    (fn {prems, context = ctxt, ...} => 
-    let
-      val _ = prems |> map @{print tracing}
-    in
-      unfold_thms_tac ctxt [rrel_F'_def] THEN
-      HEADGOAL (rtac ctxt (unfold_thms ctxt @{thms inf.idem} 
-        (unfold_thms ctxt [mr_rel_F_def, F_map_id] F_strong
-         OF (map (fn prem => unfold_thms ctxt [rrel_F'_def] prem) prems))))
-    end) ctxt)
-\<close>
-
+(*
 lemma F'_strong:
   assumes "rrel_F' R x x'" 
     and "rrel_F' Q x x'"
@@ -950,7 +695,7 @@ lemma F'_strong:
           unfolded inf.idem])
     done
   done
-
+*)
 mrbnf "('a::var, 'b::var, 'c::var, 'd) F'"
   map: map_F'
   sets: free: set1_F' bound: set2_F' bound: set3_F' live: set4_F'
